shallow embedding of dtt

experiments/DeeperShallowEmbedding.fst
@@ -9,29 +9,48 @@ val ctx : Type u#(4+1)
 let ctx = Type u#4
 
 val typ : ctx -> Type u#(4+1)
-let typ (cs :ctx) = cs -> Type u#4
+let typ cs = cs -> Type u#4
 
+(**
 let typ0 = fun (cs:ctx) -> cs -> Type u#0
 let typ1 = fun (cs:ctx) -> cs -> Type u#1
 let typ2 = fun (cs:ctx) -> cs -> Type u#2
 let typ3 = fun (cs:ctx) -> cs -> Type u#3
-
-val term : (cs : ctx) -> typ cs -> Type u#4
-let term cs t = (c:cs) -> t c
+**)
 
 val empty_ctx : ctx
-let empty_ctx : ctx = raise_t empty // or true?
-val cons : (cs : ctx) -> typ cs -> ctx
-let cons cs t = 
-  cs * (c:cs -> t c)
+let empty_ctx : ctx = raise_t unit // or true?
 
-val var : (cs : ctx)  -> typ cs -> Type u#4
+val cons : cs:ctx -> typ cs -> ctx
+let cons cs t = 
+  c:cs & t c
+
+val var : cs:ctx  -> typ cs -> Type u#4
 let var cs t = (c:cs) -> t c
 
-val weakenT : (#cs : ctx)  -> (#t : typ cs) -> typ cs -> typ (cons cs t)
-let weakenT t (c, _) = t c
+val weakenT : #cs:ctx -> #t:(typ cs) -> typ cs -> typ (cons cs t)
+let weakenT t (| c, _ |) = t c
 
-val same : (#cs : ctx)  -> (#t : typ cs) -> var (cons cs t) (weakenT t)
-let same = 
-  // TODO: fails here
-  fun (c, small_t) -> small_t
+val same : #cs:ctx -> #at:(typ cs) -> var (cons cs at) (weakenT at)
+let same = fun (| _, a |) -> a
+
+val next : #cs:ctx -> #t:(typ cs) -> #at:(typ cs) -> var cs at -> var (cons cs t) (weakenT at)
+let next x = fun (| c, _ |) -> x c
+
+val dt : #cs:ctx -> at:(typ cs) -> bt:(typ (cons cs at)) -> typ cs
+let dt #cs at bt = fun (c:cs) -> ((a : at c) -> bt (| c, a |))
+
+val u : #cs:ctx -> typ cs
+let u c = Type
+
+val term : cs:ctx -> typ cs -> Type u#4
+let term cs t = (c:cs) -> t c
+
+val lookup : #cs:ctx -> #t:(typ cs) -> icx:(var cs t) -> term cs t
+let lookup x = x
+
+val lambda : #cs:ctx -> #at:(typ cs) -> #bt:(typ (cons cs at)) -> term (cons cs at) bt -> term cs (dt at bt)
+let lambda e = fun c a -> e (| c, a |)
+
+val app : #cs:ctx -> #at:(typ cs) -> #bt:(typ (cons cs at)) -> term cs (dt at bt) -> (a : term cs at) -> term cs (fun c -> bt (| c, a c |))
+let app e1 e2 = fun c -> (e1 c) (e2 c)
